rename files and prove main function

clightplus_examples/xorlist/xorlist1.v
@@ -79,14 +79,14 @@ Section PROP.
   Proof. des_ifs. Qed.
 
 
-  Definition full_xorlist q hd_hdl tl_hdl xs : iProp :=
-    (∃ m_hd_hdl m_tl_hdl hd tl ofs_hd_hdl ofs_tl_hdl tg_hd_hdl tg_tl_hdl,
+  Definition full_xorlist q hd_hdl tl_hdl tg_hd_hdl tg_tl_hdl xs : iProp :=
+    (∃ m_hd_hdl m_tl_hdl hd tl ofs_hd_hdl ofs_tl_hdl,
     hd_hdl (↦_m_hd_hdl,q) (encode_val Mptr hd)
     ** hd_hdl (⊨_m_hd_hdl,tg_hd_hdl,q) ofs_hd_hdl
-    ** ⌜((size_chunk Mptr) | Ptrofs.unsigned ofs_hd_hdl)%Z⌝
+    ** ⌜m_hd_hdl.(sz) = size_chunk Mptr /\ ((size_chunk Mptr) | Ptrofs.unsigned ofs_hd_hdl)%Z⌝
     ** tl_hdl (↦_m_tl_hdl,q) (encode_val Mptr tl)
     ** tl_hdl (⊨_m_tl_hdl,tg_tl_hdl,q) ofs_tl_hdl
-    ** ⌜((size_chunk Mptr) | Ptrofs.unsigned ofs_tl_hdl)%Z⌝
+    ** ⌜m_tl_hdl.(sz) = size_chunk Mptr /\ ((size_chunk Mptr) | Ptrofs.unsigned ofs_tl_hdl)%Z⌝
     ** frag_xorlist q m_null m_null Vnullptr hd tl Vnullptr xs)%I.
 
   (* Example xorlist_example1 q p1 p2 p3 m1 m2 m3 i1 i2 i3:
@@ -353,42 +353,42 @@ Section SPEC.
 
   Definition add_hd_spec : fspec :=
     (mk_simple
-      (fun '(hd_handler, tl_handler, item, xs) => (
+      (fun '(hd_handler, tl_handler, tg_hd_hdl, tg_tl_hdl, item, xs) => (
         (ord_pure 1%nat),
         (fun varg => ⌜varg = [hd_handler; tl_handler; Vlong item]↑⌝
-                     ** full_xorlist 1 hd_handler tl_handler xs),
+                     ** full_xorlist 1 hd_handler tl_handler tg_hd_hdl tg_tl_hdl xs),
         (fun vret => ⌜vret = Vundef↑⌝
-                     ** full_xorlist 1 hd_handler tl_handler (Vlong item :: xs))
+                     ** full_xorlist 1 hd_handler tl_handler tg_hd_hdl tg_tl_hdl (Vlong item :: xs))
     )))%I.
 
   Definition add_tl_spec : fspec :=
     (mk_simple
-      (fun '(hd_handler, tl_handler, item, xs) => (
+      (fun '(hd_handler, tl_handler, tg_hd_hdl, tg_tl_hdl, item, xs) => (
         (ord_pure 1%nat),
         (fun varg => ⌜varg = [hd_handler; tl_handler; Vlong item]↑⌝
-                     ** full_xorlist 1 hd_handler tl_handler xs),
+                     ** full_xorlist 1 hd_handler tl_handler tg_hd_hdl tg_tl_hdl xs),
         (fun vret => ⌜vret = Vundef↑⌝
-                     ** full_xorlist 1 hd_handler tl_handler (xs ++ [Vlong item]))
+                     ** full_xorlist 1 hd_handler tl_handler tg_hd_hdl tg_tl_hdl (xs ++ [Vlong item]))
     )))%I.
 
   Definition delete_hd_spec : fspec :=
     (mk_simple
-      (fun '(hd_handler, tl_handler, xs) => (
+      (fun '(hd_handler, tl_handler, tg_hd_hdl, tg_tl_hdl, xs) => (
         (ord_pure 1%nat),
         (fun varg => ⌜varg = [hd_handler; tl_handler]↑⌝
-                     ** full_xorlist 1 hd_handler tl_handler xs),
+                     ** full_xorlist 1 hd_handler tl_handler tg_hd_hdl tg_tl_hdl xs),
         (fun vret => let '(item, xs') := vlist_delete_hd xs (Vlong Int64.zero) in
-                     ⌜vret = item↑⌝ ** full_xorlist 1 hd_handler tl_handler xs')
+                     ⌜vret = item↑⌝ ** full_xorlist 1 hd_handler tl_handler tg_hd_hdl tg_tl_hdl xs')
     )))%I.
 
   Definition delete_tl_spec : fspec :=
     (mk_simple
-      (fun '(hd_handler, tl_handler, xs) => (
+      (fun '(hd_handler, tl_handler, tg_hd_hdl, tg_tl_hdl, xs) => (
         (ord_pure 1%nat),
         (fun varg => ⌜varg = [hd_handler; tl_handler]↑⌝
-                     ** full_xorlist 1 hd_handler tl_handler xs),
+                     ** full_xorlist 1 hd_handler tl_handler tg_hd_hdl tg_tl_hdl xs),
         (fun vret => let '(item, xs') := vlist_delete_tl xs (Vlong Int64.zero) in
-                     ⌜vret = item↑⌝ ** full_xorlist 1 hd_handler tl_handler xs')
+                     ⌜vret = item↑⌝ ** full_xorlist 1 hd_handler tl_handler tg_hd_hdl tg_tl_hdl xs')
     )))%I.
 
   (* Definition search_spec : fspec :=
@@ -441,20 +441,4 @@ Section SMOD.
      ("delete_tl", mk_pure delete_tl_spec)
      ].
   
-  Definition SxorSem : SModSem.t := {|
-    SModSem.fnsems := xorSbtb;
-    SModSem.mn := "xorlist";
-    SModSem.initial_mr := ε;
-    SModSem.initial_st := tt↑;
-  |}.
-
-  Variable xor0: Mod.t.
-
-  Definition Sxor : SMod.t := {|
-    SMod.get_modsem := fun _ => SxorSem;
-    SMod.sk := xor0.(Mod.sk);
-  |}.
-
-  Definition xor stb : Mod.t := (SMod.to_tgt stb) Sxor.
-
 End SMOD.
