clightplus_examples/xorlist/xorlistall1.v
@@ -1,0 +1,40 @@
+Require Import CoqlibCCR.
+Require Import Skeleton.
+Require Import PCM.
+Require Import HoareDef.
+Require Import ProofMode.
+Require Import STB.
+Require Import Any.
+Require Import ModSem.
+Require Import ModSemE.
+Require Import ClightPlusMem1.
+Require Import xorlistall0.
+Require Import xorlist1.
+Require Import main1.
+(* From compcert Require Export Ctypes Values AST Memdata Integers. *)
+
+Set Implicit Arguments.
+Section SMOD.
+
+  Context `{@GRA.inG pointstoRA Σ}.
+  Context `{@GRA.inG allocatedRA Σ}.
+  Context `{@GRA.inG blocksizeRA Σ}.
+  Context `{@GRA.inG blockaddressRA Σ}.
+
+  Definition SxorAllSem : SModSem.t := {|
+    SModSem.fnsems := firstn 2 xorlist1.xorSbtb ++ main1.mainSbtb ++ drop 2 xorlist1.xorSbtb ;
+    SModSem.mn := "xorlist";
+    SModSem.initial_mr := ε;
+    SModSem.initial_st := tt↑;
+  |}.
+
+  Definition SxorAll : SMod.t := {|
+    SMod.get_modsem := fun _ => SxorAllSem;
+    SMod.sk := xor_sk;
+  |}.
+
+  Definition xorAllWraped stb : Mod.t := (SMod.to_tgt stb) SxorAll.
+
+  Definition xorAll : Mod.t := SMod.to_src SxorAll.
+
+End SMOD.
